camkes: Shuffle some helper lemmas around; labels as strings.
Moves some unnecessary stuff out of the locale and now specifies the label type
as `string` rather than a locale parameter. The purpose of the latter is to
allow us to talk about concrete labels rather than continually falling back on
the user's projection, but it's not clear yet whether this is a big win.

camkes/cdl-refine/Generator_CAMKES_CDL.thy
@@ -44,6 +44,17 @@ definition sum :: "nat list \<Rightarrow> nat"
 definition enumerate' :: "word32 \<Rightarrow> 'a list \<Rightarrow> (word32 \<times> 'a) list"
   where "enumerate' start xs = map (\<lambda>(a, b). (of_nat a, b)) (enumerate (unat start) xs)"
 
+definition
+  lop :: "nat \<Rightarrow> 'a list \<Rightarrow> 'a list"
+where
+  "lop n xs \<equiv> take (length xs - n) xs"
+
+abbreviation behead
+  where "behead s pref \<equiv> drop (length pref) s"
+
+abbreviation trunc
+  where "trunc s suf \<equiv> lop (length suf) s"
+
 (* Cap rights *)
 abbreviation "G \<equiv> {AllowGrant}"
 abbreviation "R \<equiv> {AllowRead}"
@@ -73,33 +84,6 @@ where
      (\<forall>x \<in> ran (irqs_objects irqs). case x of
         Types_D.CNode c \<Rightarrow> c = \<lparr>cdl_cnode_caps = empty, cdl_cnode_size_bits = 0\<rparr>
       | _ \<Rightarrow> False)"
-
-text {*
-  We assume that the user, when instantiating the following locale to use the contained lemmas, will
-  provide us with a function to find the object IDs of the IPC buffers. We need to assume this
-  because the IPC buffer frames (and caps to them) are inferred late in the CapDL generation
-  process, while deriving the rest of the backing frames for the address space.
-*}
-locale cdl_translation =
-  fixes ipc_buffer :: "string \<Rightarrow> nat \<Rightarrow> cdl_object_id option"
-  assumes buffers_distinct: "\<And>n i m j. \<exists>f. ipc_buffer n i = Some f \<and> ipc_buffer m j = Some f
-                               \<Longrightarrow> n = m \<and> i = j"
-  fixes id_of :: "string \<Rightarrow> cdl_object_id option"
-  assumes ids_distinct: "\<And>n m. \<exists>i. id_of n = Some i \<and> id_of m = Some i \<Longrightarrow> n = m"
-begin
-
-abbreviation the_ipc_buffer :: "string \<Rightarrow> nat \<Rightarrow> cdl_object_id"
-  where "the_ipc_buffer name index \<equiv> the (ipc_buffer name index)"
-
-abbreviation the_id_of :: "string \<Rightarrow> cdl_object_id"
-  where "the_id_of name \<equiv> the (id_of name)"
-
-abbreviation the_cnode_of :: "string \<Rightarrow> cdl_object_id"
-  where "the_cnode_of instance \<equiv> the_id_of (''cnode_'' @ instance)"
-
-(* XXX: Assumes no shared address space components. *)
-abbreviation the_pd_of :: "string \<Rightarrow> cdl_object_id"
-  where "the_pd_of instance \<equiv> the_id_of (''pd_'' @ instance @ ''_group_bin'')"
 
 text {*
   Predicate that the extra capability distribution we provide to the @{text generate} function is a
@@ -172,6 +156,193 @@ definition cap_offset :: "camkes_state \<Rightarrow> string \<Rightarrow> nat"
     (\<lambda>(_, c). length (requires c) + length (provides c) + length (dataports c) +
               length (emits c) + length (consumes c))
       (hd (filter (\<lambda>(n, _). n = instance) (components (composition spec))))"
+
+lemma helper1: "map (length \<circ> (\<lambda>(a, b). P a b # map (f a b) (Q a b))) xs =
+                  map (\<lambda>(a, b). 1 + length (Q a b)) xs"
+  by clarsimp
+
+lemma helper2: "(\<Sum>x \<leftarrow> xs. Suc (f x)) = length xs + (\<Sum>x \<leftarrow> xs. f x)"
+  apply (induct xs)
+   by clarsimp+
+
+lemma helper3: "(\<Sum>(a, b) \<leftarrow> xs. Suc (f a b)) = length xs + (\<Sum>(a, b) \<leftarrow> xs. f a b)"
+  apply (induct xs)
+   by clarsimp+
+
+lemma helper4: "fold op + ((map (\<lambda>(a, b). f a b) xs)::nat list) 0 = (\<Sum>(a, b) \<leftarrow> xs. f a b)"
+  apply (subst fold_plus_listsum_rev)
+  apply (subst listsum_rev)
+  by clarsimp
+
+lemma set_of_enumerate:"card (set (enumerate n xs)) = length xs"
+  by (metis distinct_card distinct_enumerate length_enumerate)
+
+lemma collapse_fst:"fst ` (\<lambda>x. (f x, g x)) ` s = f ` s"
+  by force
+
+lemma collapse_fst2:"fst ` (\<lambda>(x, y). (f x, g y)) ` s = (\<lambda>x. f (fst x)) ` s"
+  by force
+
+lemma collapse_fst3:"(\<lambda>x. f (fst x)) ` set (enumerate n xs) = f ` set [n..<n + length xs]"
+  by (metis image_image list.set_map map_fst_enumerate)
+
+lemma card_of_dom_bounded:
+  fixes f :: "'a \<Rightarrow> 'b option"
+  assumes "finite (UNIV::'a set)"
+  shows "card (dom f) \<le> CARD('a)"
+  by (metis assms card_seteq linear top_greatest)
+
+lemma helper8: "x \<in> f ` S = (\<exists>y \<in> S. f y = x)"
+  by blast
+
+lemma helper7:
+  "n \<le> CARD(cdl_object_id) \<Longrightarrow> card ((of_nat::nat \<Rightarrow> cdl_object_id) ` {0..<n}) = card {0..<n}"
+  apply clarsimp
+  apply (induct n)
+   apply clarsimp+
+  apply (subgoal_tac "{0..<Suc n} = {0..<n} \<union> {n}")
+   prefer 2
+   apply clarsimp
+   apply fastforce
+  apply clarsimp
+  apply (subst card_insert_disjoint)
+    apply clarsimp
+   apply (subst atLeast0LessThan)
+   apply (subgoal_tac "(of_nat::nat \<Rightarrow> cdl_object_id) ` {..<n} = {..<of_nat n}")
+    prefer 2
+    apply (rule equalityI)
+     apply clarsimp
+     apply (subst (asm) card_word)
+     apply clarsimp
+     apply (rule of_nat_mono_maybe)
+      apply clarsimp+
+      apply (subst helper8)
+      apply (rule bexI) (* sorry for schematics *)
+       apply (rule word_unat.Rep_inverse')
+       apply force
+      apply clarsimp 
+      apply (subst (asm) card_word)
+      apply clarsimp
+      apply (metis (erased, hide_lams) Divides.mod_less_eq_dividend order_less_le_trans unat_of_nat word_less_nat_alt)
+     by clarsimp+
+
+lemma helper6: "n \<le> CARD(cdl_object_id) \<Longrightarrow> card ((of_nat::nat \<Rightarrow> cdl_object_id) ` {0..<n}) = n"
+  apply (subst helper7)
+   by clarsimp+
+
+lemma third_in: "(a, b, c) \<in> S \<Longrightarrow> c \<in> (snd \<circ> snd) ` S"
+  by (metis (erased, hide_lams) helper8 image_comp snd_conv)
+
+lemma helper9: "(a \<in> (snd \<circ> snd) ` (set (enumerate i xs))) = (a \<in> snd ` (set xs))"
+  by (metis map_map map_snd_enumerate set_map)
+
+abbreviation "is_some s \<equiv> \<not> Option.is_none s"
+
+lemma helper11: "is_some (map_of (enumerate' n xs) x) \<Longrightarrow> \<exists>y. map_of (enumerate' n xs) x = Some y"
+  by (metis (full_types) is_none_code(1) not_Some_eq)
+
+lemma helper10: "map_of (enumerate' n xs) x = Some y \<Longrightarrow> y \<in> set xs"
+  apply (clarsimp simp:enumerate'_def)
+  by (metis enumerate_eq_zip in_set_zipE map_of_SomeD zip_map1)
+
+lemma helper14:
+  "(map_of xs ++ map_of ys) x = (case map_of ys x of None \<Rightarrow> map_of xs x | Some x' \<Rightarrow> Some x')"
+  apply (case_tac "(map_of xs ++ map_of ys) x")
+   apply clarsimp+
+  apply (case_tac "map_of ys x")
+   by clarsimp+
+
+lemma helper15:
+  "(map_of xs ++ map_of ys ++ map_of zs) x =
+     (case map_of zs x of None \<Rightarrow> (case map_of ys x of None \<Rightarrow> map_of xs x
+                                                     | Some x' \<Rightarrow> Some x')
+                        | Some x' \<Rightarrow> Some x')"
+  apply (case_tac "(map_of xs ++ map_of ys ++ map_of zs) x")
+   apply clarsimp+
+  apply (case_tac "map_of zs x")
+   apply clarsimp
+   apply (case_tac "map_of ys x")
+    by clarsimp+
+
+lemma helper13: "map_of (map (\<lambda>(n, y). (the_id_of n, y)) xs) x = Some z \<Longrightarrow> z \<in> snd ` set xs"
+  proof -
+    assume "map_of (map (\<lambda>(n, y). (the_id_of n, y)) xs) x = Some z"
+    hence "(x, z) \<in> (\<lambda>(uu, y). (the_id_of uu, y)) ` set xs" using map_of_SomeD by fastforce
+    thus "z \<in> snd ` set xs" using helper8 by fastforce
+  qed
+
+lemma helper12: "valid_extra a b \<Longrightarrow> dom (cdl_objects a) \<inter> dom b = {}"
+  by (clarsimp simp:valid_extra_def)
+
+lemma helper16: "(a, b) \<in> set (enumerate x ys) \<Longrightarrow> b \<in> set ys"
+  by (metis enumerate_eq_zip in_set_zip2)
+
+lemma helper17: "distinct (map fst xs) \<Longrightarrow> ran (map_of xs) = set (map snd xs)"
+  apply (cut_tac xs="map fst xs" and ys="map snd xs" in ran_map_of_zip[symmetric])
+    apply clarsimp+
+  by (simp add: ran_distinct)
+
+lemma helper18: "x \<in> ran (map_of xs) \<Longrightarrow> x \<in> set (map snd xs)"
+  by (metis (mono_tags, hide_lams) helper8 map_of_SomeD ranE set_map snd_conv)
+
+lemma helper19: "x \<in> ran (xs ++ ys ++ zs) \<Longrightarrow> x \<in> ran xs \<or> x \<in> ran ys \<or> x \<in> ran zs"
+  by (smt map_add_Some_iff ranE ranI)
+
+lemma helper21: "None \<notin> S \<Longrightarrow> Some x \<in> S = (x \<in> the ` S)"
+  apply (rule iffI)
+   apply force
+  apply (subst in_these_eq[symmetric])
+  apply (clarsimp simp:these_def)
+  apply (case_tac "\<exists>y. xa = Some y")
+   by clarsimp+
+
+lemma helper20: "the ` Set.filter (\<lambda>s. \<not> Option.is_none s) (range f) = ran f"
+  apply (rule subset_antisym)
+   apply clarsimp
+   apply (case_tac "f x", simp_all)
+   apply (simp add: ranI)
+  apply clarsimp
+  apply (subst helper21[symmetric])
+   apply clarsimp+
+  apply (erule ranE)
+  by (metis range_eqI)
+
+lemma helper23:
+  "x \<in> ran (cdl_objects (merge_objs a b)) \<Longrightarrow> x \<in> ran (cdl_objects a) \<or> x \<in> ran b"
+  apply (clarsimp simp:merge_objs_def merge_cdl_def)
+  by (metis helper19 map_add_id)
+
+type_synonym label = string
+
+text {*
+  We assume that the user, when instantiating the following locale to use the contained lemmas, will
+  provide us with a function to find the object IDs of the IPC buffers. We need to assume this
+  because the IPC buffer frames (and caps to them) are inferred late in the CapDL generation
+  process, while deriving the rest of the backing frames for the address space.
+*}
+locale cdl_translation =
+  fixes ipc_buffer :: "string \<Rightarrow> nat \<Rightarrow> cdl_object_id option"
+  assumes buffers_distinct: "\<And>n i m j. \<exists>f. ipc_buffer n i = Some f \<and> ipc_buffer m j = Some f
+                               \<Longrightarrow> n = m \<and> i = j"
+  fixes id_of :: "string \<Rightarrow> cdl_object_id option"
+  assumes ids_distinct: "\<And>n m. \<exists>i. id_of n = Some i \<and> id_of m = Some i \<Longrightarrow> n = m"
+
+  fixes garbage :: label
+  fixes irq_label :: label
+begin
+
+abbreviation the_ipc_buffer :: "string \<Rightarrow> nat \<Rightarrow> cdl_object_id"
+  where "the_ipc_buffer name index \<equiv> the (ipc_buffer name index)"
+
+abbreviation the_id_of :: "string \<Rightarrow> cdl_object_id"
+  where "the_id_of name \<equiv> the (id_of name)"
+
+abbreviation the_cnode_of :: "string \<Rightarrow> cdl_object_id"
+  where "the_cnode_of instance \<equiv> the_id_of (''cnode_'' @ instance)"
+
+(* XXX: Assumes no shared address space components. *)
+abbreviation the_pd_of :: "string \<Rightarrow> cdl_object_id"
+  where "the_pd_of instance \<equiv> the_id_of (''pd_'' @ instance @ ''_group_bin'')"
 
 text {*
   The contents of a CNode of a given component instance. It is easier to define this out-of-line
@@ -260,23 +431,6 @@ where
 
      (components (composition spec)))"
 
-lemma helper1: "map (length \<circ> (\<lambda>(a, b). P a b # map (f a b) (Q a b))) xs =
-                  map (\<lambda>(a, b). 1 + length (Q a b)) xs"
-  by clarsimp
-
-lemma helper2: "(\<Sum>x \<leftarrow> xs. Suc (f x)) = length xs + (\<Sum>x \<leftarrow> xs. f x)"
-  apply (induct xs)
-   by clarsimp+
-
-lemma helper3: "(\<Sum>(a, b) \<leftarrow> xs. Suc (f a b)) = length xs + (\<Sum>(a, b) \<leftarrow> xs. f a b)"
-  apply (induct xs)
-   by clarsimp+
-
-lemma helper4: "fold op + ((map (\<lambda>(a, b). f a b) xs)::nat list) 0 = (\<Sum>(a, b) \<leftarrow> xs. f a b)"
-  apply (subst fold_plus_listsum_rev)
-  apply (subst listsum_rev)
-  by clarsimp
-
 lemma tcb_count_correct: "tcb_count spec = length (tcb_objs spec)"
   apply (clarsimp simp:tcb_count_def tcb_objs_def sum_def)
   apply (subst length_concat)
@@ -298,64 +452,8 @@ where
 definition obj_heap_size :: "camkes_state \<Rightarrow> nat"
   where "obj_heap_size spec \<equiv> cnode_count spec + tcb_count spec + ep_count spec"
 
-lemma set_of_enumerate:"card (set (enumerate n xs)) = length xs"
-  by (metis distinct_card distinct_enumerate length_enumerate)
-
-lemma collapse_fst:"fst ` (\<lambda>x. (f x, g x)) ` s = f ` s"
-  by force
-
-lemma collapse_fst2:"fst ` (\<lambda>(x, y). (f x, g y)) ` s = (\<lambda>x. f (fst x)) ` s"
-  by force
-
-lemma collapse_fst3:"(\<lambda>x. f (fst x)) ` set (enumerate n xs) = f ` set [n..<n + length xs]"
-  by (metis image_image list.set_map map_fst_enumerate)
-
-lemma card_of_dom_bounded:
-  fixes f :: "'a \<Rightarrow> 'b option"
-  assumes "finite (UNIV::'a set)"
-  shows "card (dom f) \<le> CARD('a)"
-  by (metis assms card_seteq linear top_greatest)
-
 lemma obj_heap_dom_bounded:"card (dom (obj_heap spec)) \<le> CARD(cdl_object_id)"
   apply (rule card_mono[where B=UNIV])
-   by clarsimp+
-
-lemma helper8: "x \<in> f ` S = (\<exists>y \<in> S. f y = x)"
-  by blast
-
-lemma helper7:
-  "n \<le> CARD(cdl_object_id) \<Longrightarrow> card ((of_nat::nat \<Rightarrow> cdl_object_id) ` {0..<n}) = card {0..<n}"
-  apply clarsimp
-  apply (induct n)
-   apply clarsimp+
-  apply (subgoal_tac "{0..<Suc n} = {0..<n} \<union> {n}")
-   prefer 2
-   apply clarsimp
-   apply fastforce
-  apply clarsimp
-  apply (subst card_insert_disjoint)
-    apply clarsimp
-   apply (subst atLeast0LessThan)
-   apply (subgoal_tac "(of_nat::nat \<Rightarrow> cdl_object_id) ` {..<n} = {..<of_nat n}")
-    prefer 2
-    apply (rule equalityI)
-     apply clarsimp
-     apply (subst (asm) card_word)
-     apply clarsimp
-     apply (rule of_nat_mono_maybe)
-      apply clarsimp+
-      apply (subst helper8)
-      apply (rule bexI) (* sorry for schematics *)
-       apply (rule word_unat.Rep_inverse')
-       apply force
-      apply clarsimp 
-      apply (subst (asm) card_word)
-      apply clarsimp
-      apply (metis (erased, hide_lams) Divides.mod_less_eq_dividend order_less_le_trans unat_of_nat word_less_nat_alt)
-     by clarsimp+
-
-lemma helper6: "n \<le> CARD(cdl_object_id) \<Longrightarrow> card ((of_nat::nat \<Rightarrow> cdl_object_id) ` {0..<n}) = n"
-  apply (subst helper7)
    by clarsimp+
 
 text {* Low-level generator. This describes the actual logic of the CAmkES code generator. *}
@@ -372,8 +470,158 @@ where
      cdl_current_domain = undefined\<rparr>"
 
 text {*
-  Top-level generator. We validate the capability extension and then use the low-level generator
-  above.
+  An object abstraction (that is, a mapping from object IDs to labels) for a CAmkES-generated
+  specification. WIP.
+*}
+definition
+  poa_of :: "camkes_state \<Rightarrow> cdl_heap \<Rightarrow> irqs \<Rightarrow> label agent_map"
+where
+  "poa_of spec extra irqs \<equiv> (\<lambda>id. case (
+
+     (* Labelling of the output of the low-level generator: *)
+     fold (op ++)
+       (map (\<lambda>(name, _). [the_id_of name \<mapsto> behead name ''cnode_'']) (cnode_objs spec))
+         Map.empty
+
+     ++
+     fold (op ++)
+       (map (\<lambda>(name, _). [the_id_of name \<mapsto> trunc name ''_ep'']) (ep_objs spec)) Map.empty
+     ++
+     fold (op ++)
+       (map (\<lambda>(name, _). [the_id_of name \<mapsto> behead name ''tcb_'']) (tcb_objs spec)) Map.empty
+
+     (* Labelling of address space objects: *)
+     ++
+     (\<lambda>id. case extra id of
+             Some _ \<Rightarrow> if \<exists>name. id_of name = Some id
+                          then Some (trunc
+                                      (behead (SOME name. id_of name = Some id) ''frame_'')
+                                        ''_group_bin_0000'')
+                          else None
+           | None \<Rightarrow> None)
+
+     (* Labelling of IRQ objects: *)
+     ++
+     (\<lambda>id. if id \<in> dom (irqs_objects irqs)
+              then Some irq_label
+              else None)
+
+     ) id of Some l \<Rightarrow> l | None \<Rightarrow> garbage)"
+
+abbreviation "edge_subject \<equiv> fst"
+abbreviation "edge_auth \<equiv> fst o snd"
+abbreviation "edge_object \<equiv> snd o snd"
+
+text {*
+  A policy describing the authority between labels in a CapDL system. Note that the only meaningful
+  relationships here are the authority implied by endpoints. TODO: shared memory.
+*}
+definition
+  policy_of :: "camkes_state \<Rightarrow> cdl_heap \<Rightarrow> irqs \<Rightarrow> label auth_graph"
+where
+  "policy_of spec extra irqs \<equiv>
+     (* Every label has every authority over itself. *)
+     {edge. edge_subject edge = edge_object edge} \<union>
+
+     (* Senders on seL4RPC connections. *)
+     {edge. \<exists>from. from \<in> fst ` set (components (composition spec)) \<and>
+                   (\<exists>conn \<in> set (connections (composition spec)).
+                      fst (conn_from (snd conn)) = from \<and>
+                      conn_type (snd conn) = seL4RPC \<and>
+                      edge_object edge = fst conn) \<and>
+                    edge_subject edge = from \<and>
+                    edge_auth edge \<in> {Receive, Reset, SyncSend}} \<union>
+
+     (* Receivers on seL4RPC connections. *)
+     {edge. \<exists>to. to \<in> fst ` set (components (composition spec)) \<and>
+                 (\<exists>conn \<in> set (connections (composition spec)).
+                    fst (conn_to (snd conn)) = to \<and>
+                    conn_type (snd conn) = seL4RPC \<and>
+                    edge_object edge = fst conn) \<and>
+                  edge_subject edge = to \<and>
+                  edge_auth edge \<in> {Receive, Reset, SyncSend}} \<union>
+
+     (* Senders on seL4Asynch connections. *)
+     {edge. \<exists>from. from \<in> fst ` set (components (composition spec)) \<and>
+                   (\<exists>conn \<in> set (connections (composition spec)).
+                      fst (conn_from (snd conn)) = from \<and>
+                      conn_type (snd conn) = seL4Asynch \<and>
+                      edge_object edge = fst conn) \<and>
+                    edge_subject edge = from \<and>
+                    edge_auth edge \<in> {AsyncSend, Reset}} \<union>
+
+     (* Receivers on seL4Asynch connections. *)
+     {edge. \<exists>to. to \<in> fst ` set (components (composition spec)) \<and>
+                 (\<exists>conn \<in> set (connections (composition spec)).
+                    fst (conn_to (snd conn)) = to \<and>
+                    conn_type (snd conn) = seL4Asynch \<and>
+                    edge_object edge = fst conn) \<and>
+                  edge_subject edge = to \<and>
+                  edge_auth edge \<in> {Receive, Reset}}"
+
+lemma pw_decompose:
+  "\<lbrakk>\<forall>agent. (\<forall>agent'. (agent, Control, agent') \<in> aag \<longrightarrow> agent = agent')
+         \<and> (\<forall>a. (agent, a, agent) \<in> aag);
+    \<exists>agent. policy_wellformed aag mirqs irqs agent\<rbrakk>
+    \<Longrightarrow> \<forall>agent. policy_wellformed aag False irqs agent"
+  by (clarsimp simp:policy_wellformed_def)
+
+lemma no_trans_grant: "subj = obj \<or> (subj, Grant, obj) \<notin> policy_of spec extras irqs"
+  by (clarsimp simp:policy_of_def)
+
+lemma pw_control:
+  "\<lbrakk>policy_wellformed policy mirqs irqs l; (s, Receive, l) \<in> policy\<rbrakk> \<Longrightarrow> (l, Control, s) \<in> policy"
+  apply (rule_tac ep=l and mirqs=mirqs and irqs=irqs and l=l in aag_wellformed_grant_Control_to_recv)
+    apply (rule_tac mirqs=mirqs and irqs=irqs in aag_wellformed_refl)
+    by assumption+
+
+lemma pw_control':
+  "\<lbrakk>policy_wellformed policy mirqs irqs l; (s, Receive, l) \<in> policy\<rbrakk> \<Longrightarrow> (s, Control, l) \<in> policy"
+  apply (rule_tac ep=l and mirqs=mirqs and irqs=irqs and l=l in aag_wellformed_grant_Control_to_send)
+    apply (rule_tac mirqs=mirqs and irqs=irqs in aag_wellformed_refl)
+    by assumption+
+
+lemma pw_same_label:
+  "\<lbrakk>policy_wellformed policy mirqs irqs l; (s, Receive, l) \<in> policy\<rbrakk> \<Longrightarrow> s = l"
+  apply (frule_tac s=s in pw_control, assumption)
+  apply (frule_tac s=s in pw_control', assumption)
+  apply (rule sym)
+  apply (rule_tac aag=policy and mirqs=mirqs and irqs=irqs in aag_wellformed_Control)
+   by assumption+
+
+lemma policy_wf: "wellformed_assembly spec \<Longrightarrow>
+    \<forall>agent. policy_wellformed (policy_of spec extras irqs) False {irq_label} agent"
+  apply (clarsimp simp:policy_wellformed_def)
+  apply (rule conjI)
+   apply (clarsimp simp:policy_of_def)
+  apply (rule conjI)
+   apply (clarsimp simp:policy_of_def)
+  apply clarsimp
+  apply (rename_tac subj subj' obj)
+  apply (cut_tac subj=subj and obj=obj and spec=spec and extras=extras and irqs=irqs in no_trans_grant)
+  apply clarsimp
+  oops
+
+(* TODO *)
+definition
+  pas_of :: "camkes_state \<Rightarrow> cdl_heap \<Rightarrow> irqs \<Rightarrow> label PAS set"
+where
+  "pas_of spec extra irqs \<equiv> {pas.
+     pasObjectAbs pas = poa_of spec extra irqs \<and>
+     (\<forall>asid. pasASIDAbs pas asid = garbage) \<and>
+     (\<forall>irq. pasIRQAbs pas irq = irq_label) \<and>
+     pasPolicy pas = policy_of spec extra irqs \<and>
+     pasSubject pas \<notin> {garbage, irq_label} \<and>
+     \<not> pasMayActivate pas \<and>
+     \<not> pasMayEditReadyQueues pas \<and>
+     \<not> pasMaySendIrqs pas \<and>
+     (\<forall>domain. (domain = 0 \<and> pasDomainAbs pas domain \<noteq> garbage) \<or>
+               (domain \<noteq> 0 \<and> pasDomainAbs pas domain = garbage))
+   }"
+
+text {*
+  Top-level state generator. We validate the capability extension and then use the low-level
+  generator above.
 *}
 definition
   state_of :: "camkes_state \<Rightarrow> cdl_heap \<Rightarrow> irqs \<Rightarrow> cdl_state option"
@@ -399,7 +647,6 @@ lemma merge_contained:
      \<Longrightarrow> cdl_objects x u = Some v \<or> cdl_objects y u = Some v"
   by (clarsimp simp:merge_cdl_def)
 
-abbreviation "is_some s \<equiv> \<not> Option.is_none s"
 abbreviation "obj_ids cdl \<equiv> dom (cdl_objects cdl)"
 abbreviation "obj_ids' extra \<equiv> dom extra"
 abbreviation "obj_count cdl \<equiv> card (obj_ids cdl)"
@@ -425,49 +672,10 @@ lemma tcb_objs_only_tcbs: "\<forall>(_, i) \<in> set (tcb_objs spec). case i of 
   apply (erule disjE)                                       
    by clarsimp+
 
-lemma third_in: "(a, b, c) \<in> S \<Longrightarrow> c \<in> (snd \<circ> snd) ` S"
-  by (metis (erased, hide_lams) helper8 image_comp snd_conv)
-
-lemma helper9: "(a \<in> (snd \<circ> snd) ` (set (enumerate i xs))) = (a \<in> snd ` (set xs))"
-  by (metis map_map map_snd_enumerate set_map)
-
 lemma ep_objs_only_eps:
   "\<forall>(_, i) \<in> set (ep_objs spec). case i of Types_D.Endpoint \<Rightarrow> True | Types_D.AsyncEndpoint \<Rightarrow> True | _ \<Rightarrow> False"
   apply (clarsimp simp:ep_objs_def ep_objs'_def)
   by (metis cdl_object.simps(98) cdl_object.simps(99))
-
-lemma helper11: "is_some (map_of (enumerate' n xs) x) \<Longrightarrow> \<exists>y. map_of (enumerate' n xs) x = Some y"
-  by (metis (full_types) is_none_code(1) not_Some_eq)
-
-lemma helper10: "map_of (enumerate' n xs) x = Some y \<Longrightarrow> y \<in> set xs"
-  apply (clarsimp simp:enumerate'_def)
-  by (metis enumerate_eq_zip in_set_zipE map_of_SomeD zip_map1)
-
-lemma helper14:
-  "(map_of xs ++ map_of ys) x = (case map_of ys x of None \<Rightarrow> map_of xs x | Some x' \<Rightarrow> Some x')"
-  apply (case_tac "(map_of xs ++ map_of ys) x")
-   apply clarsimp+
-  apply (case_tac "map_of ys x")
-   by clarsimp+
-
-lemma helper15:
-  "(map_of xs ++ map_of ys ++ map_of zs) x =
-     (case map_of zs x of None \<Rightarrow> (case map_of ys x of None \<Rightarrow> map_of xs x
-                                                     | Some x' \<Rightarrow> Some x')
-                        | Some x' \<Rightarrow> Some x')"
-  apply (case_tac "(map_of xs ++ map_of ys ++ map_of zs) x")
-   apply clarsimp+
-  apply (case_tac "map_of zs x")
-   apply clarsimp
-   apply (case_tac "map_of ys x")
-    by clarsimp+
-
-lemma helper13: "map_of (map (\<lambda>(n, y). (the_id_of n, y)) xs) x = Some z \<Longrightarrow> z \<in> snd ` set xs"
-  proof -
-    assume "map_of (map (\<lambda>(n, y). (the_id_of n, y)) xs) x = Some z"
-    hence "(x, z) \<in> (\<lambda>(uu, y). (the_id_of uu, y)) ` set xs" using map_of_SomeD by fastforce
-    thus "z \<in> snd ` set xs" using helper8 by fastforce
-  qed
 
 lemma generated_no_pds_pts_frames:
   "generate' spec = cdl \<Longrightarrow>
@@ -506,9 +714,6 @@ lemma generated_no_pds_pts_frames:
    apply clarsimp
    by (case_tac b', simp_all)
 
-lemma helper12: "valid_extra a b \<Longrightarrow> dom (cdl_objects a) \<inter> dom b = {}"
-  by (clarsimp simp:valid_extra_def)
-
 lemma generated_objects_disjoint:
   "state_of spec extra irqs = Some cdl \<Longrightarrow>
      obj_count (generate' spec) + obj_count' extra + obj_count' (irqs_objects irqs) = obj_count cdl"
@@ -529,9 +734,6 @@ lemma generated_objects_disjoint:
   apply (clarsimp simp:state_of_def merge_cdl_def merge_objs_def)
   by (simp add: Un_assoc)
 
-lemma helper16: "(a, b) \<in> set (enumerate x ys) \<Longrightarrow> b \<in> set ys"
-  by (metis enumerate_eq_zip in_set_zip2)
-
 lemma only_endpoint_caps:
   "\<forall>cap \<in> ran (cap_map a xs). case cap of Types_D.EndpointCap _ _ _ \<Rightarrow> True
                                         | Types_D.AsyncEndpointCap _ _ _ \<Rightarrow> True
@@ -544,41 +746,6 @@ lemma only_endpoint_caps:
   apply (rename_tac connection irrelevant)
   apply (case_tac "conn_type connection = seL4RPC", simp_all)
    by (case_tac "from_component connection = xs", simp_all)+
-
-lemma helper17: "distinct (map fst xs) \<Longrightarrow> ran (map_of xs) = set (map snd xs)"
-  apply (cut_tac xs="map fst xs" and ys="map snd xs" in ran_map_of_zip[symmetric])
-    apply clarsimp+
-  by (simp add: ran_distinct)
-
-lemma helper18: "x \<in> ran (map_of xs) \<Longrightarrow> x \<in> set (map snd xs)"
-  by (metis (mono_tags, hide_lams) helper8 map_of_SomeD ranE set_map snd_conv)
-
-lemma helper19: "x \<in> ran (xs ++ ys ++ zs) \<Longrightarrow> x \<in> ran xs \<or> x \<in> ran ys \<or> x \<in> ran zs"
-  by (smt map_add_Some_iff ranE ranI)
-
-lemma helper21: "None \<notin> S \<Longrightarrow> Some x \<in> S = (x \<in> the ` S)"
-  apply (rule iffI)
-   apply force
-  apply (subst in_these_eq[symmetric])
-  apply (clarsimp simp:these_def)
-  apply (case_tac "\<exists>y. xa = Some y")
-   by clarsimp+
-
-lemma helper20: "the ` Set.filter (\<lambda>s. \<not> Option.is_none s) (range f) = ran f"
-  apply (rule subset_antisym)
-   apply clarsimp
-   apply (case_tac "f x", simp_all)
-   apply (simp add: ranI)
-  apply clarsimp
-  apply (subst helper21[symmetric])
-   apply clarsimp+
-  apply (erule ranE)
-  by (metis range_eqI)
-
-lemma helper23:
-  "x \<in> ran (cdl_objects (merge_objs a b)) \<Longrightarrow> x \<in> ran (cdl_objects a) \<or> x \<in> ran b"
-  apply (clarsimp simp:merge_objs_def merge_cdl_def)
-  using helper19 by force
 
 lemma valid_only_empty_cnodes:
   "valid_irqs spec extra irqs \<Longrightarrow> \<forall>obj \<in> ran (irqs_objects irqs). case obj of
@@ -661,6 +828,21 @@ lemma generated_caps_limited:
   apply (erule_tac x=cnode in ballE)
    apply (case_tac cnode; simp_all)
   by clarsimp
+
+text {* Compose the functions for producing a state and PAS into a single top-level generator. *}
+definition
+  generate :: "camkes_state \<Rightarrow> cdl_heap \<Rightarrow> irqs \<Rightarrow> (cdl_state \<times> label PAS set) option"
+where
+  "generate spec extra irqs \<equiv>
+     case state_of spec extra irqs of Some state \<Rightarrow> Some (state, pas_of spec extra irqs)
+                                    | None \<Rightarrow> None"
+
+lemma "\<lbrakk>generate spec extra irqs = Some (state, pases); pas \<in> pases;
+        (subject, Control, object) \<in> pasPolicy pas\<rbrakk>
+         \<Longrightarrow> subject = object"
+  apply (clarsimp simp:generate_def pas_of_def policy_of_def)
+  apply (case_tac "state_of spec extra irqs"; clarsimp)+
+  done
 
 end
 
